src/Helpers/BigOp.v
@@ -1,5 +1,4 @@
-From iris.proofmode Require Import coq_tactics reduction.
-From iris.algebra Require Import auth gmap frac agree excl vector.
+From iris.algebra Require Import gmap.
 From Perennial.goose_lang Require Import proofmode.
 
 Lemma big_sepM2_lookup_1_some
@@ -56,4 +55,51 @@ Proof.
   case_eq (m1 !! i); auto.
   iIntros (? ? ?) "H".
   iDestruct (big_sepM2_lookup_1 with "H") as (x1) "[% _]"; eauto; congruence.
+Qed.
+
+Lemma loc_add_Sn l n :
+  l +ₗ S n = (l +ₗ 1) +ₗ n.
+Proof.
+  rewrite loc_add_assoc.
+  f_equal.
+  lia.
+Qed.
+
+Theorem heap_array_to_list {Σ} {A} l0 (vs: list A) (P: loc -> A -> iProp Σ) :
+  ([∗ map] l↦v ∈ heap_array l0 vs, P l v) ⊣⊢
+  ([∗ list] i↦v ∈ vs, P (l0 +ₗ i) v).
+Proof.
+  (iInduction (vs) as [| v vs] "IH" forall (l0)).
+  - simpl.
+    rewrite big_sepM_empty.
+    auto.
+  - simpl.
+    rewrite loc_add_0.
+    rewrite big_sepM_union.
+    { rewrite big_sepM_singleton.
+      setoid_rewrite loc_add_Sn.
+      iSpecialize ("IH" $! (l0 +ₗ 1)).
+      iSplit.
+      + iIntros "($&Hm)".
+        iApply ("IH" with "Hm").
+      + iIntros "($&Hl)".
+        iApply ("IH" with "Hl").
+    }
+    symmetry.
+    apply heap_array_map_disjoint; intros.
+    apply (not_elem_of_dom (D := gset loc)).
+    rewrite dom_singleton.
+    intros ?%elem_of_singleton.
+    rewrite loc_add_assoc in H2.
+    apply loc_add_ne in H2; auto; lia.
+Qed.
+
+Theorem big_sepL_impl {Σ} A (f g: nat -> A -> iProp Σ) (l: list A) :
+  (forall i x, f i x -∗ g i x) ->
+  ([∗ list] i↦x ∈ l, f i x) -∗
+  ([∗ list] i↦x ∈ l, g i x).
+Proof.
+  intros Himpl.
+  apply big_opL_gen_proper; auto.
+  typeclasses eauto.
 Qed.
