src/program_proof/append_log_proof.v
@@ -1,6 +1,7 @@
 From Perennial.goose_lang.examples Require Import append_log.
 From Perennial.goose_lang.lib Require Import encoding.
 From Perennial.program_proof Require Import proof_prelude.
+From Perennial.program_proof Require Import disk_lib.
 From Perennial.program_proof Require Import marshal_proof.
 
 Section heap.
@@ -11,106 +12,9 @@ Implicit Types z : Z.
 Implicit Types s : Slice.t.
 Implicit Types (stk:stuckness) (E: coPset).
 
-Lemma byte_ptsto_untype l q (x: u8) :
-  l ↦[byteT]{q} #x ⊣⊢ l ↦{q} #x.
-Proof.
-  rewrite /struct_mapsto /=.
-  rewrite loc_add_0 right_id.
-  iSplit.
-  - iDestruct 1 as "[$ _]".
-  - iDestruct 1 as "$".
-    auto.
-Qed.
-
-Lemma array_to_block_array l q b :
-  array l q byteT (Block_to_vals b) ⊣⊢ mapsto_block l q b.
-Proof.
-  rewrite /mapsto_block /array.
-  rewrite heap_array_to_list.
-  rewrite ?big_sepL_fmap.
-  setoid_rewrite Z.mul_1_l.
-  apply big_opL_proper.
-  intros k y Heq.
-  rewrite /Block_to_vals in Heq.
-  rewrite /b2val.
-  rewrite byte_ptsto_untype //.
-Qed.
-
 Local Opaque struct_mapsto load_ty store_ty.
 
-Lemma slice_to_block_array s q b :
-  is_slice_small s byteT q (Block_to_vals b) -∗ mapsto_block s.(Slice.ptr) q b.
-Proof.
-  iIntros "[Ha _]".
-  by iApply array_to_block_array.
-Qed.
-
-Lemma block_array_to_slice l q b cap :
-  mapsto_block l q b -∗ is_slice_small (Slice.mk l 4096 cap) byteT q (Block_to_vals b).
-Proof.
-  iIntros "Hm".
-  iSplitL.
-  { by iApply array_to_block_array. }
-  iPureIntro.
-  rewrite length_Block_to_vals.
-  simpl.
-  reflexivity.
-Qed.
-
 Notation length := strings.length.
-
-Transparent disk.Read disk.Write.
-
-Theorem wp_Write stk E (a: u64) s q b :
-  {{{ ▷ ∃ b0, int.val a d↦ b0 ∗ is_slice_small s byteT q (Block_to_vals b) }}}
-    Write #a (slice_val s) @ stk; E
-  {{{ RET #(); int.val a d↦ b ∗ is_slice_small s byteT q (Block_to_vals b) }}}.
-Proof.
-  iIntros (Φ) ">Hpre HΦ".
-  iDestruct "Hpre" as (b0) "[Hda Hs]".
-  wp_call.
-  wp_call.
-  iDestruct (is_slice_small_sz with "Hs") as %Hsz.
-  wp_apply (wp_WriteOp with "[Hda Hs]").
-  { iIntros "!>".
-    iExists b0.
-    iFrame.
-    by iApply slice_to_block_array. }
-  iIntros "[Hda Hmapsto]".
-  iApply "HΦ".
-  iFrame.
-  iSplitL; auto.
-  by iApply array_to_block_array.
-Qed.
-
-Theorem wp_Write' stk E (z: Z) (a: u64) s q b :
-  {{{ ⌜int.val a = z⌝ ∗ ▷ ∃ b0, z d↦ b0 ∗ is_slice_small s byteT q (Block_to_vals b) }}}
-    Write #a (slice_val s) @ stk; E
-  {{{ RET #(); z d↦ b ∗ is_slice_small s byteT q (Block_to_vals b) }}}.
-Proof.
-  iIntros (Φ) "[<- >Hpre] HΦ".
-  iApply (wp_Write with "[$Hpre]").
-  eauto.
-Qed.
-
-Lemma wp_Read stk E (a: u64) q b :
-  {{{ ▷ int.val a d↦{q} b }}}
-    Read #a @ stk; E
-  {{{ s, RET slice_val s;
-      int.val a d↦{q} b ∗
-      is_slice s byteT 1%Qp (Block_to_vals b) }}}.
-Proof.
-  iIntros (Φ) ">Hda HΦ".
-  wp_call.
-  wp_apply (wp_ReadOp with "Hda").
-  iIntros (l) "(Hda&Hl)".
-  iDestruct (block_array_to_slice _ _ _ 4096 with "Hl") as "Hs".
-  wp_pures.
-  wp_apply (wp_raw_slice with "Hs").
-  iIntros (s) "Hs".
-  iApply "HΦ".
-  iFrame.
-Qed.
 
 Definition is_hdr_block (sz disk_sz: u64) (b: Block) :=
   ∃ (extra: list u8), Block_to_vals b = b2val <$> encode [EncUInt64 sz; EncUInt64 disk_sz] ++ extra.
@@ -132,86 +36,6 @@ Definition is_log (v:val) (vs:list Block): iProp Σ :=
    is_log' sz disk_sz vs.
 
 Open Scope Z.
-
-Theorem wpc_Write stk k E1 E2 (a: u64) s q b :
-  {{{ ▷ ∃ b0, int.val a d↦ b0 ∗ is_slice_small s byteT q (Block_to_vals b) }}}
-    Write #a (slice_val s) @ stk; k; E1; E2
-  {{{ RET #(); int.val a d↦ b ∗ is_slice_small s byteT q (Block_to_vals b) }}}
-  {{{ ∃ b', int.val a d↦ b' ∗ is_slice_small s byteT q (Block_to_vals b) }}}.
-Proof.
-  iIntros (Φ Φc) ">Hpre HΦ".
-  iDestruct "Hpre" as (b0) "[Hda Hs]".
-  rewrite /Write /slice.ptr.
-  wpc_pures.
-  { iExists b0; iFrame. }
-  iDestruct (is_slice_small_sz with "Hs") as %Hsz.
-  wpc_atomic.
-  { iExists b0; iFrame. }
-  wp_apply (wp_WriteOp with "[Hda Hs]").
-  { iIntros "!>".
-    iExists b0; iFrame.
-    by iApply slice_to_block_array. }
-  iIntros "[Hda Hmapsto]".
-  iSplit.
-  - iModIntro; crash_case.
-    iExists b; iFrame.
-    destruct s; simpl in Hsz.
-    replace sz with (U64 4096).
-    + by iApply block_array_to_slice.
-    + rewrite length_Block_to_vals in Hsz.
-      change block_bytes with (Z.to_nat 4096) in Hsz.
-      apply word.unsigned_inj.
-      word.
-  - iApply "HΦ".
-    iFrame.
-    iSplitL; auto.
-    by iApply array_to_block_array.
-Qed.
-
-Theorem wpc_Write' stk k E1 E2 (a: u64) s q b0 b :
-  {{{ ▷ int.val a d↦ b0 ∗ is_slice_small s byteT q (Block_to_vals b) }}}
-    Write #a (slice_val s) @ stk; k; E1; E2
-  {{{ RET #(); int.val a d↦ b ∗ is_slice_small s byteT q (Block_to_vals b) }}}
-  {{{ (int.val a d↦ b0 ∨ int.val a d↦ b) ∗ is_slice_small s byteT q (Block_to_vals b) }}}.
-Proof.
-  iIntros (Φ Φc) "[>Hda Hs] HΦ".
-  rewrite /Write /slice.ptr.
-  wpc_pures; iFrame.
-  iDestruct (is_slice_small_sz with "Hs") as %Hsz.
-  wpc_atomic; iFrame.
-  wp_apply (wp_WriteOp with "[Hda Hs]").
-  { iIntros "!>".
-    iExists b0; iFrame.
-    by iApply slice_to_block_array. }
-  iIntros "[Hda Hmapsto]".
-  iSplit.
-  - iModIntro; crash_case; iFrame.
-    destruct s; simpl in Hsz.
-    replace sz with (U64 4096).
-    + by iApply block_array_to_slice.
-    + rewrite length_Block_to_vals in Hsz.
-      change block_bytes with (Z.to_nat 4096) in Hsz.
-      apply word.unsigned_inj.
-      word.
-  - iApply "HΦ".
-    iFrame.
-    iSplitL; auto.
-    by iApply array_to_block_array.
-Qed.
-
-Theorem slice_to_block s q bs :
-  s.(Slice.sz) = 4096 ->
-  is_slice_small s byteT q (b2val <$> bs) -∗
-  mapsto_block s.(Slice.ptr) q (list_to_block bs).
-Proof.
-  iIntros (Hsz) "Hs".
-  iDestruct "Hs" as "[Hl %]".
-  rewrite fmap_length in H.
-  iApply (array_to_block with "Hl").
-  assert (int.val (Slice.sz s) = 4096).
-  { rewrite Hsz. reflexivity. }
-  lia.
-Qed.
 
 Theorem wp_mkHdr stk E (sz disk_sz:u64) :
   {{{ True }}}
