src/program_proof/disk_lib.v
@@ -1,0 +1,232 @@
+From Perennial.program_proof Require Import proof_prelude.
+
+Section goose.
+Context `{!heapG Σ}.
+Context `{!crashG Σ}.
+Implicit Types v : val.
+Implicit Types z : Z.
+Implicit Types s : Slice.t.
+Implicit Types (stk:stuckness) (E: coPset).
+
+Definition list_to_block (l: list u8) : Block :=
+  match decide (length l = Z.to_nat 4096) with
+  | left H => eq_rect _ _ (list_to_vec l) _ H
+  | _ => inhabitant
+  end.
+
+Lemma vec_to_list_of_list_eq_rect A (l: list A) n (H: length l = n) :
+  vec_to_list (eq_rect _ _ (list_to_vec l) _ H) = l.
+Proof.
+  rewrite <- H; simpl.
+  rewrite vec_to_list_of_list.
+  auto.
+Qed.
+
+Definition list_to_block_to_vals l :
+  length l = Z.to_nat 4096 ->
+  Block_to_vals (list_to_block l) = b2val <$> l.
+Proof.
+  intros H.
+  rewrite /list_to_block /Block_to_vals.
+  rewrite decide_left.
+  f_equal.
+  rewrite vec_to_list_of_list_eq_rect; auto.
+Qed.
+
+Lemma array_to_block l q (bs: list byte) :
+  length bs = Z.to_nat 4096 ->
+  l ↦∗[byteT]{q} (b2val <$> bs) -∗ mapsto_block l q (list_to_block bs).
+Proof.
+  rewrite /array /mapsto_block /Block_to_vals /list_to_block.
+  iIntros (H) "Hl".
+  rewrite decide_left.
+  rewrite heap_array_to_list.
+  rewrite !big_sepL_fmap.
+  rewrite vec_to_list_of_list_eq_rect.
+  setoid_rewrite Z.mul_1_l.
+  iApply (big_sepL_impl with "Hl"); simpl.
+  iModIntro.
+  iIntros (i x) "% [Hl _]".
+  simpl.
+  rewrite loc_add_0 right_id /b2val.
+  iFrame.
+Qed.
+
+Lemma byte_ptsto_untype l q (x: u8) :
+  l ↦[byteT]{q} #x ⊣⊢ l ↦{q} #x.
+Proof.
+  rewrite /struct_mapsto /=.
+  rewrite loc_add_0 right_id.
+  iSplit.
+  - iDestruct 1 as "[$ _]".
+  - iDestruct 1 as "$".
+    auto.
+Qed.
+
+Lemma array_to_block_array l q b :
+  array l q byteT (Block_to_vals b) ⊣⊢ mapsto_block l q b.
+Proof.
+  rewrite /mapsto_block /array.
+  rewrite heap_array_to_list.
+  rewrite ?big_sepL_fmap.
+  setoid_rewrite Z.mul_1_l.
+  apply big_opL_proper.
+  intros k y Heq.
+  rewrite /Block_to_vals in Heq.
+  rewrite /b2val.
+  rewrite byte_ptsto_untype //.
+Qed.
+
+Lemma slice_to_block_array s q b :
+  is_slice_small s byteT q (Block_to_vals b) -∗ mapsto_block s.(Slice.ptr) q b.
+Proof.
+  iIntros "[Ha _]".
+  by iApply array_to_block_array.
+Qed.
+
+Lemma block_array_to_slice l q b cap :
+  mapsto_block l q b -∗ is_slice_small (Slice.mk l 4096 cap) byteT q (Block_to_vals b).
+Proof.
+  iIntros "Hm".
+  iSplitL.
+  { by iApply array_to_block_array. }
+  iPureIntro.
+  rewrite length_Block_to_vals.
+  simpl.
+  reflexivity.
+Qed.
+
+Transparent disk.Read disk.Write.
+
+Theorem wp_Write stk E (a: u64) s q b :
+  {{{ ▷ ∃ b0, int.val a d↦ b0 ∗ is_slice_small s byteT q (Block_to_vals b) }}}
+    Write #a (slice_val s) @ stk; E
+  {{{ RET #(); int.val a d↦ b ∗ is_slice_small s byteT q (Block_to_vals b) }}}.
+Proof.
+  iIntros (Φ) ">Hpre HΦ".
+  iDestruct "Hpre" as (b0) "[Hda Hs]".
+  wp_call.
+  wp_call.
+  iDestruct (is_slice_small_sz with "Hs") as %Hsz.
+  wp_apply (wp_WriteOp with "[Hda Hs]").
+  { iIntros "!>".
+    iExists b0.
+    iFrame.
+    by iApply slice_to_block_array. }
+  iIntros "[Hda Hmapsto]".
+  iApply "HΦ".
+  iFrame.
+  iSplitL; auto.
+  by iApply array_to_block_array.
+Qed.
+
+Theorem wp_Write' stk E (z: Z) (a: u64) s q b :
+  {{{ ⌜int.val a = z⌝ ∗ ▷ ∃ b0, z d↦ b0 ∗ is_slice_small s byteT q (Block_to_vals b) }}}
+    Write #a (slice_val s) @ stk; E
+  {{{ RET #(); z d↦ b ∗ is_slice_small s byteT q (Block_to_vals b) }}}.
+Proof.
+  iIntros (Φ) "[<- >Hpre] HΦ".
+  iApply (wp_Write with "[$Hpre]").
+  eauto.
+Qed.
+
+Lemma wp_Read stk E (a: u64) q b :
+  {{{ ▷ int.val a d↦{q} b }}}
+    Read #a @ stk; E
+  {{{ s, RET slice_val s;
+      int.val a d↦{q} b ∗
+      is_slice s byteT 1%Qp (Block_to_vals b) }}}.
+Proof.
+  iIntros (Φ) ">Hda HΦ".
+  wp_call.
+  wp_apply (wp_ReadOp with "Hda").
+  iIntros (l) "(Hda&Hl)".
+  iDestruct (block_array_to_slice _ _ _ 4096 with "Hl") as "Hs".
+  wp_pures.
+  wp_apply (wp_raw_slice with "Hs").
+  iIntros (s) "Hs".
+  iApply "HΦ".
+  iFrame.
+Qed.
+
+Theorem wpc_Write stk k E1 E2 (a: u64) s q b :
+  {{{ ▷ ∃ b0, int.val a d↦ b0 ∗ is_slice_small s byteT q (Block_to_vals b) }}}
+    Write #a (slice_val s) @ stk; k; E1; E2
+  {{{ RET #(); int.val a d↦ b ∗ is_slice_small s byteT q (Block_to_vals b) }}}
+  {{{ ∃ b', int.val a d↦ b' ∗ is_slice_small s byteT q (Block_to_vals b) }}}.
+Proof.
+  iIntros (Φ Φc) ">Hpre HΦ".
+  iDestruct "Hpre" as (b0) "[Hda Hs]".
+  rewrite /Write /slice.ptr.
+  wpc_pures.
+  { iExists b0; iFrame. }
+  iDestruct (is_slice_small_sz with "Hs") as %Hsz.
+  wpc_atomic.
+  { iExists b0; iFrame. }
+  wp_apply (wp_WriteOp with "[Hda Hs]").
+  { iIntros "!>".
+    iExists b0; iFrame.
+    by iApply slice_to_block_array. }
+  iIntros "[Hda Hmapsto]".
+  iSplit.
+  - iModIntro; crash_case.
+    iExists b; iFrame.
+    destruct s; simpl in Hsz.
+    replace sz with (U64 4096).
+    + by iApply block_array_to_slice.
+    + rewrite length_Block_to_vals in Hsz.
+      change block_bytes with (Z.to_nat 4096) in Hsz.
+      apply word.unsigned_inj.
+      word.
+  - iApply "HΦ".
+    iFrame.
+    iSplitL; auto.
+    by iApply array_to_block_array.
+Qed.
+
+Theorem wpc_Write' stk k E1 E2 (a: u64) s q b0 b :
+  {{{ ▷ int.val a d↦ b0 ∗ is_slice_small s byteT q (Block_to_vals b) }}}
+    Write #a (slice_val s) @ stk; k; E1; E2
+  {{{ RET #(); int.val a d↦ b ∗ is_slice_small s byteT q (Block_to_vals b) }}}
+  {{{ (int.val a d↦ b0 ∨ int.val a d↦ b) ∗ is_slice_small s byteT q (Block_to_vals b) }}}.
+Proof.
+  iIntros (Φ Φc) "[>Hda Hs] HΦ".
+  rewrite /Write /slice.ptr.
+  wpc_pures; iFrame.
+  iDestruct (is_slice_small_sz with "Hs") as %Hsz.
+  wpc_atomic; iFrame.
+  wp_apply (wp_WriteOp with "[Hda Hs]").
+  { iIntros "!>".
+    iExists b0; iFrame.
+    by iApply slice_to_block_array. }
+  iIntros "[Hda Hmapsto]".
+  iSplit.
+  - iModIntro; crash_case; iFrame.
+    destruct s; simpl in Hsz.
+    replace sz with (U64 4096).
+    + by iApply block_array_to_slice.
+    + rewrite length_Block_to_vals in Hsz.
+      change block_bytes with (Z.to_nat 4096) in Hsz.
+      apply word.unsigned_inj.
+      word.
+  - iApply "HΦ".
+    iFrame.
+    iSplitL; auto.
+    by iApply array_to_block_array.
+Qed.
+
+Theorem slice_to_block s q bs :
+  s.(Slice.sz) = 4096 ->
+  is_slice_small s byteT q (b2val <$> bs) -∗
+  mapsto_block s.(Slice.ptr) q (list_to_block bs).
+Proof.
+  iIntros (Hsz) "Hs".
+  iDestruct "Hs" as "[Hl %]".
+  rewrite fmap_length in H.
+  iApply (array_to_block with "Hl").
+  assert (int.val (Slice.sz s) = 4096).
+  { rewrite Hsz. reflexivity. }
+  lia.
+Qed.
+
+End goose.
